Rework array abstractions to fit new semantic model.

rocq-osiris/theories/program_logic/rules/array_rules.v
@@ -1,5 +1,6 @@
 From iris Require Import gen_heap proofmode.proofmode.
 From osiris Require Import lang.
+From osiris.tactics Require Import osiris_utils.
 From osiris.program_logic Require Import ewp.
 From osiris.program_logic.rules Require Import impure_rules stop_rules.
 From osiris.logic Require Import list_z big_opLZ.
@@ -15,43 +16,64 @@ Section array_resources.
 
   Context `{!osirisGS Σ}.
 
-  Definition isArray (a : array) (n : Z) : iProp Σ :=
-    ∃ t ls, pointsto a DfracDiscarded (Dict t ls) ∗
-            ⌜length ls = n⌝ ∗ ⌜0 ≤ n ≤ max_array⌝.
+  Definition isArray (a : array) (ls : list loc) : iProp Σ :=
+    ∃ t, pointsto a DfracDiscarded (Dict t ls) ∗
+         ⌜length ls ≤ max_array⌝.
 
-  Global Instance is_array_persistent a n : Persistent (isArray a n).
+  Global Instance is_array_persistent a ls : Persistent (isArray a ls).
   Proof. apply _. Qed.
 
-  Definition isSlice `{Encode A} dq (a : array) (i : Z) (xs : list A) : iProp Σ :=
-    ∃ t ls, pointsto a DfracDiscarded (Dict t ls) ∗
-            ⌜0 ≤ i⌝ ∧ ⌜i + length xs ≤ length ls⌝ ∗
-            [∗ listZ] l;x ∈ seg i (i + length xs) ls; xs, l ↦{dq} #x.
+  Lemma isArray_valid a ls1 ls2 :
+    isArray a ls1 -∗ isArray a ls2 -∗ ⌜ls2 = ls1⌝.
+  Proof.
+    iIntros "(%t & #Ha & _) (% & #Ha' & _)".
+    iPoseProof (pointsto_valid_2 with "Ha Ha'") as "[_ %Heq]".
+    by inversion_clear Heq.
+  Qed.
 
-  Definition ownArray `{Encode A} (a : array) (xs : list A) : iProp Σ :=
-    isArray a (length xs) ∗ isSlice (DfracOwn 1) a 0 xs.
+  Definition isSlice `{Encode A} a dq (i : Z) (xs : list A) : iProp Σ :=
+    ∃ ls, isArray a ls ∗
+    ⌜0 ≤ i⌝ ∧ ⌜i + length xs ≤ length ls⌝ ∗
+    [∗ listZ] l;x ∈ seg i (i + length xs) ls; xs, l ↦{dq} #x.
+
+  Definition ownArray `{Encode A} (a : array) dq (xs : list A) : iProp Σ :=
+    ∃ ls, isArray a ls ∗ isSlice a dq 0 xs ∗ ⌜length ls = length xs⌝.
+
+  Lemma ownArray_isArray `{Encode A} a dq (xs : list A) :
+    ownArray a dq xs -∗ ∃ ls, isArray a ls ∗ ⌜length ls = length xs⌝.
+  Proof. iIntros "(%ls & #$ & _ & $)". Qed.
+
+  Lemma ownArray_isSlice `{Encode A} a dq (xs : list A) :
+    ownArray a dq xs -∗ isSlice a dq 0 xs.
+  Proof. iIntros "(%ls & #Ha & $ & %Hlen)". Qed.
+
+  Lemma isSlice_ownArray `{Encode A} a dq ls (xs : list A) :
+    isArray a ls -∗
+    isSlice a dq 0 xs -∗
+    ⌜length ls = length xs⌝ -∗
+    ownArray a dq xs.
+  Proof. iIntros "Ha $ $". iFrame. Qed.
 
 End array_resources.
 
 Notation "a ↦∗ dq xs" :=
-    (isSlice dq a 0 xs)
+    (ownArray a dq xs)
       (at level 20, dq custom dfrac at level 1, format "a  ↦∗ dq  xs") : bi_scope.
 Notation "a ↦∗[ i ] dq xs" :=
-  (isSlice dq a i xs)
+  (isSlice a dq i xs)
     (at level 20, dq custom dfrac at level 1, i at level 200, format "a  ↦∗[ i ] dq  xs") : bi_scope.
 
 Section array_resources.
 
-  Context `{!osirisGS Σ}.
-
-  Lemma Slice_app `{Encode A} j dq a i (xs ys : list A) :
+  Lemma Slice_app `{!osirisGS Σ} `{Encode A} j dq a i (xs ys : list A) :
     j = i + length xs →
     a ↦∗[i]{dq} (xs ++ ys) ⊣⊢ (a ↦∗[i]{dq} xs ∗ a ↦∗[j]{dq} ys).
   Proof.
     intros ->.
     lengths.
-    iStartProof; iSplit; iIntros "Hslice".
-    - iDestruct "Hslice" as "(%t & %ls & #Ha & %Hpos & %Hlen & Hls)".
-      iFrame "#". length in Hlen. length.
+    iSplit; iIntros "Hslice".
+    - iDestruct "Hslice" as "(%ls & #$ & %Hpos & %Hlen & Hls)".
+      length in Hlen. length.
       rewrite (split_seg (i + length xs)); try lia.
       iPoseProof (big_sepLZ2_app_inv with "Hls")
         as "($ & Hslice2)"; first (length; lia).
@@ -60,18 +82,15 @@ Section array_resources.
       iPureIntro. lia.
 
     - iDestruct "Hslice" as "(Hslice1 & Hslice2)".
-      iDestruct "Hslice1" as "(%t & %ls & #Ha & %Hpos & %Hlen & Hslice1)".
-      iDestruct "Hslice2" as "(%t' & %ls' & #Ha' & %Hpos' & %Hlen' & Hslice2)".
-
-      iPoseProof (pointsto_valid_2 with "Ha Ha'") as "(_ & %Heq)".
-      inversion_clear Heq.
-
-      unfold isSlice. length.
+      iDestruct "Hslice1" as "(%ls & #Harr & %Hpos & %Hlen & Hslice1)".
+      iDestruct "Hslice2" as "(% & #Harr' & %Hpos' & %Hlen' & Hslice2)".
+      iPoseProof (isArray_valid with "Harr Harr'") as "->".
+      iFrame "#". length.
 
       iPoseProof (big_sepLZ2_app with "Hslice1 Hslice2") as "Hslice".
       rewrite -(split_seg (i + length xs)); try lia.
       replace (i + (length xs + length ys)) with (i + length xs + length ys) by lia.
-      iFrame "∗#%".
+      iFrame "∗%".
   Qed.
 
   (* We can split a slice on an index [j] of the model [xs].
@@ -79,21 +98,16 @@ Section array_resources.
      This results in two slices with models
      [seg 0 j xs] and [seg j (length xs) xs]. *)
 
-  Lemma split_Slice `{Encode A} (j : Z) dq a i (xs : list A) :
+  Lemma split_Slice `{!osirisGS Σ} `{Encode A} (j : Z) dq ls i (xs : list A) :
     0 ≤ j ≤ length xs →
-    a ↦∗[i]{dq} xs ⊣⊢ a ↦∗[i]{dq} (seg 0 j xs) ∗ a ↦∗[i + j]{dq} (seg j (length xs) xs).
+    ls ↦∗[i]{dq} xs ⊣⊢ ls ↦∗[i]{dq} (seg 0 j xs) ∗ ls ↦∗[i + j]{dq} (seg j (length xs) xs).
   Proof.
     lengths.
     rewrite -{1}(seg_all 0 (length xs) xs); try lia.
     rewrite (split_seg j); try lia.
-    rewrite (Slice_app (i + j)).
-    reflexivity. length. lia.
+    rewrite (Slice_app (i + j)). reflexivity.
+    length; lia.
   Qed.
-
-  Lemma slice_of_own `{Encode A} (a : array) (xs : list A) n :
-    n = length xs →
-    ownArray a xs ⊣⊢ isArray a n ∗ a ↦∗ xs.
-   Proof. intros ->. done. Qed.
 
 End array_resources.
 
@@ -104,42 +118,86 @@ Section array_reasoning.
 
   Context {η : env} {E : coPset} {Ψ : iEff Σ}.
 
-  Lemma imp_as_array {ζ} (m : microvx) (Φ : array → iProp Σ) :
-    imp m @ E <|Ψ|> ⟨⟨ ζ ⟩⟩ {{ Φ }} -∗
+  Global Instance notval_listloc : NotVal (list loc) := {}.
+
+  (** General [as_array] rule.  Given that the postcondition of [m] implies
+      [isArray a ls] for some [a] and [ls], the [load_block] step is
+      discharged automatically and [Φ ls] is delivered. *)
+  Lemma imp_as_array {ζ} {Φ : list loc → iProp Σ} (Φ1 : loc → iProp Σ) (m : microvx) :
+    imp m @ E <|Ψ|> ⟨⟨ ζ ⟩⟩ {{ Φ1 }} -∗
+    (∀ a, Φ1 a -∗ ∃ ls, isArray a ls ∗ Φ ls) -∗
     imp as_array m @ E <|Ψ|> ⟨⟨ ζ ⟩⟩ {{ Φ }}.
   Proof.
-    iIntros "Hm".
+    iIntros "Hm H".
     iApply (imp_bind with "Hm").
-    iIntros (a) "HΦ".
-    iApply (imp_ret with "HΦ"); encode.
+    iIntros (a) "HΦ1".
+    iDestruct ("H" with "HΦ1") as "(%ls & (%t & #Hpts & %Hbound) & HΦ)".
+    iApply (imp_load_block' with "Hpts").
+    iIntros "!> _". iExact "HΦ".
+  Qed.
+
+  (** [as_array] rule for a pre-existing array.  Use when [isArray a ls] is
+      already in context and [m] reduces to the array address [a]. *)
+  Lemma imp_as_array_isArray {ζ} {Φ : list loc → iProp Σ} a ls (m : microvx) :
+    isArray a ls -∗
+    imp m @ E <|Ψ|> ⟨⟨ ζ ⟩⟩ {{ λ a', ⌜a' = a⌝ }} -∗
+    Φ ls -∗
+    imp as_array m @ E <|Ψ|> ⟨⟨ ζ ⟩⟩ {{ Φ }}.
+  Proof.
+    iIntros "#Harr Hm HΦ".
+    iApply (imp_as_array (λ a', ⌜a' = a⌝)%I with "Hm").
+    iIntros (a') "->".
+    iExists ls. iFrame "#∗".
+  Qed.
+
+  (** [as_array] rule for a freshly allocated array.  Use when [m] allocates
+      an array, producing [ownArray a ls xs]; the full ownership is preserved
+      in the postcondition together with any additional frame [R a xs]. *)
+  Lemma imp_as_array_ownArray `{Encode A} {ζ}
+      {R : array → list A → iProp Σ} (m : microvx) :
+    imp m @ E <|Ψ|> ⟨⟨ ζ ⟩⟩ {{ λ a, ∃ (xs : list A), a ↦∗ xs ∗ R a xs }} -∗
+    imp as_array m @ E <|Ψ|> ⟨⟨ ζ ⟩⟩ {{ λ ls, ∃ a xs, a ↦∗ xs ∗ R a xs }}.
+  Proof.
+    iIntros "Hm".
+    iApply (imp_as_array (λ a, ∃ xs, a ↦∗ xs ∗ R a xs)%I with "Hm").
+    iIntros (a) "(%xs & Hown & $)".
+    iPoseProof (ownArray_isArray with "Hown") as "(%ls & #Ha & %)".
+    iFrame "Hown Ha".
   Qed.
 
   Lemma imp_EArrayLit `{Encode A} {ζ} (Φs : list (A → iProp Σ)) es :
     ⌜length Φs = length es ∧ length es ≤ max_array⌝ -∗
     imp evals η es @ E <|Ψ|> ⟨⟨ ζ ⟩⟩ {{ λ xs, [∗ listZ] x;Φ ∈ xs;Φs, Φ x }} -∗
     imp eval η (EArrayLit es) @ E <|Ψ|> ⟨⟨ ζ ⟩⟩
-      {{ λ a, ∃ xs, ownArray a xs ∗ [∗ listZ] x;Φ ∈ xs;Φs, Φ x }}.
+      {{ λ a, ∃ xs, a ↦∗ xs ∗ [∗ listZ] x;Φ ∈ xs;Φs, Φ x }}.
   Proof.
     iIntros "[%Hleneq %Hlenbound] He". simpl_eval.
     iApply (imp_bind (A1:=list A) with "He").
     iIntros (xs) "HΦs".
     iApply imp_bind.
     { iApply imp_allocn. iIntros "!>" (ls) "Hls". iExact "Hls". }
-    iIntros (arr) "Hls". iApply imp_ret; first encode.
+    iIntros (arr) "Hls".
     iPoseProof (big_sepLZ2_length with "Hls") as "%Hlenls".
     iPoseProof (big_sepLZ2_length with "HΦs") as "%Hlenxs".
-    iFrame. simpl.
-    iSplitR.
-    - iPureIntro.
-      length_nonneg es; rewrite Hlenls Hlenxs Hleneq; lia.
-    - iSplit. { iPureIntro; lia. }
-      rewrite -Hlenls.
-      by seg.
+    iApply imp_bind.
+    { iApply imp_alloc_block. }
+    iIntros (a) "#Ha".
+    iApply imp_ret; first encode.
+    iFrame "HΦs".
+
+    (* Goal: establish [a ↦∗ xs] from
+       [a ↦ (Dict Mut arr)] and [∀ l x ∈ arr xs, l ↦ #x ]. *)
+    iAssert (isArray a arr) as "#Harr".
+    { iFrame "Ha". iPureIntro.
+      rewrite Hlenls Hlenxs Hleneq. apply Hlenbound. }
+    iApply (isSlice_ownArray with "Harr [Hls] [//]").
+    iFrame "Harr". seg. iFrame "Hls".
+    iPureIntro; lia.
   Qed.
 
   Lemma imp_EArrayEmpty `{Encode A} {ζ} :
     ⊢ imp eval η (EArrayLit []) @ E <|Ψ|> ⟨⟨ ζ ⟩⟩
-        {{ λ a, ownArray a (@nil A) }}.
+        {{ λ a, a ↦∗ (@nil A) }}.
   Proof.
     iApply imp_wand.
     - iApply (imp_EArrayLit (@nil (A → _))  []).
@@ -148,20 +206,34 @@ Section array_reasoning.
       simpl_evals. iApply imp_ret; first encode.
       by iApply big_sepLZ2_nil.
     - iIntros (a) "(%xs & HownArr & Hxs)".
-      by iPoseProof (big_sepLZ2_nil_inv_r with "Hxs") as "->".
+      iDestruct "HownArr" as "(%ls & HisArr & Hslice & %Hlenls)".
+      iPoseProof (big_sepLZ2_nil_inv_r with "Hxs") as "->".
+      length in Hlenls. apply nil_length_inv in Hlenls as ->.
+      by iApply (isSlice_ownArray with "HisArr Hslice").
   Qed.
 
-  Lemma imp_EArrayLength {ζ} (n : Z) e :
-    imp eval η e @ E <|Ψ|> ⟨⟨ ζ ⟩⟩ {{ λ a, isArray a n }} -∗
-    imp eval η (EArrayLength e) @ E <|Ψ|> ⟨⟨ ζ ⟩⟩ {{ λ n', ⌜n' = n⌝ }}.
+  Lemma imp_EArrayLength' {ζ} (ls : list loc) e :
+    imp eval η e @ E <|Ψ|> ⟨⟨ ζ ⟩⟩ {{ λ a, isArray a ls }} -∗
+    imp eval η (EArrayLength e) @ E <|Ψ|> ⟨⟨ ζ ⟩⟩ {{ λ n, ⌜n = length ls⌝ }}.
   Proof.
     iIntros "He". simpl_eval.
-    iApply (imp_bind with "[He]").
-    { iApply (imp_as_array with "He"). }
-    iIntros (ls) "(%Hlen & %Hbound)".
-    change (♯ls) with ls.
-    iApply (imp_ret (VInt (repr (length ls))) (length ls)%Z). encode.
-    iPureIntro. lia.
+    iApply (imp_bind with "[He] [-]").
+    - set_postcondition (λ ls', ⌜ls'=ls⌝)%I.
+      iApply (imp_as_array with "He").
+      iIntros (a) "#Harr". by iFrame "#".
+    - iIntros (ls') "->". iApply imp_ret; first encode. auto.
+  Qed.
+
+  Lemma imp_EArrayLength `{Encode A} {ζ} dq (xs : list A) e :
+    imp eval η e @ E <|Ψ|> ⟨⟨ ζ ⟩⟩ {{ λ a, a ↦∗{dq} xs }} -∗
+    imp eval η (EArrayLength e) @ E <|Ψ|> ⟨⟨ ζ ⟩⟩ {{ λ n, ⌜n = length xs⌝ }}.
+  Proof.
+    iIntros "He". simpl_eval.
+    iApply (imp_bind with "[He] [-]").
+    - set_postcondition (λ ls, ⌜length ls = length xs⌝)%I.
+      iApply (imp_as_array with "He").
+      iIntros (?) "(%ls & $ & _ & $)".
+    - iIntros (ls) "<-". iApply imp_ret; first encode. auto.
   Qed.
 
   Lemma imp_EArrayMake `{Encode A} {ζ} {e1 e2} (n : Z) (Φ : A → iProp Σ) :
@@ -169,25 +241,29 @@ Section array_reasoning.
     imp eval η e1 @ E <|Ψ|> ⟨⟨ ζ ⟩⟩ {{ λ i, ⌜i = n⌝ }} -∗
     imp eval η e2 @ E <|Ψ|> ⟨⟨ ζ ⟩⟩ {{ Φ }} -∗
     imp eval η (EArrayMake e1 e2) @ E <|Ψ|> ⟨⟨ ζ ⟩⟩
-      {{ λ (a : array), ∃ x, Φ x ∗ ownArray a (replicate n x) }}.
+      {{ λ (a : array), ∃ x, Φ x ∗ a ↦∗ (replicate n x) }}.
   Proof.
     iIntros (Hbound) "He1 He2". simpl_eval.
     iApply (imp_bind_par with "[He1] He2").
     { iApply (imp_as_int with "He1"). }
-    iIntros (? a) "->  Hφ /=".
+    iIntros (? x) "->  Hφ /=".
     rewrite signed_repr; last representable.
     case_decide; last contradiction.
     iApply imp_bind.
     { rewrite <- fmap_replicate. iApply imp_allocn.
       iIntros "!>" (ls) "Hpts". iExact "Hpts". }
     iIntros (arr) "!> Hpts".
+    iApply imp_bind. { iApply imp_alloc_block. }
+    iIntros (a) "#Ha".
+
     iApply imp_ret; first encode.
     iPoseProof (big_sepLZ2_length with "Hpts") as "%Hlen'".
     simpl. length in Hlen'.
-    iFrame.
+    iFrame "∗#".
     iSplitR. { iPureIntro; length; lia. }
-    iSplit. { iPureIntro; length; lia. }
-    by seg.
+    iSplitL. { unfold isSlice; seg; iFrame.
+               iPureIntro; length; lia. }
+    iPureIntro; length; lia.
   Qed.
 
   Global Instance inhabited_loc : Inhabited loc.
@@ -228,79 +304,101 @@ Section array_reasoning.
       revert Hlen. length. lia.
   Qed.
 
-  Lemma imp_EArrayGet2 `{Encode A, Inhabited A} {Φ : A → iProp Σ} {ζ} (Φ1 : array → iProp Σ) (Φ2 : Z → iProp Σ) e1 e2 :
-    imp eval η e1 @ E <|Ψ|> ⟨⟨ ζ ⟩⟩ {{ λ a, Φ1 a }} -∗
-    imp eval η e2 @ E <|Ψ|> ⟨⟨ ζ ⟩⟩ {{ λ i, Φ2 i }} -∗
-    (∀ a i, Φ1 a -∗ Φ2 i -∗
-            ∃ n, isArray a n ∗
-                 ∃ dq j xs,
-                   ▷ (⌜j ≤ i⌝ ∗ ⌜i - j < length xs⌝ ∗ a ↦∗[j]{dq} xs) ∗
-                   ▷ (a ↦∗[j]{dq} xs -∗ Φ (xs !!! (i - j)))) -∗
+  Lemma imp_EArrayGet2 `{Encode A, Inhabited A} {Φ : A → iProp Σ} {ζ} (Φ2 : Z → iProp Σ) e1 e2 a ls :
+    isArray a ls -∗
+    imp eval η e1 @ E <|Ψ|> ⟨⟨ ζ ⟩⟩ {{ λ a', ⌜a'=a⌝ }} -∗
+    imp eval η e2 @ E <|Ψ|> ⟨⟨ ζ ⟩⟩ {{ Φ2 }} -∗
+    (∀ i, Φ2 i -∗
+          ∃ dq j xs,
+            ▷ (⌜j ≤ i⌝ ∗ ⌜i - j < length xs⌝ ∗ a ↦∗[j]{dq} xs) ∗
+            ▷ (a ↦∗[j]{dq} xs -∗ Φ (xs !!! (i - j)))) -∗
     imp eval η (EArrayGet e1 e2) @ E <|Ψ|> ⟨⟨ ζ ⟩⟩ {{ Φ }}.
   Proof.
-    iIntros "He1 He2 P". simpl_eval.
+    iIntros "#Ha He1 He2 P". simpl_eval.
     iApply (imp_bind_par with "[He1] [He2]").
-    { iApply (imp_as_array with "He1"). }
-    { iApply (imp_as_int with "He2"). }
-    iIntros (a i) "HΦ1 HΦ2".
-    iDestruct ("P" with "HΦ1 HΦ2") as
-      "(%n & #Harr & %dq & %j & %xs & >Hslice & Hlookup)".
-    iDestruct "Harr" as "(%Hlen' & %Hbound)".
-    iDestruct "Hslice" as "(%Hle & %Hlt & (%Hlen & Hslice))".
-    simpl.
-    rewrite signed_repr; last representable.
-    rewrite list_lookup_lookup_total_valid; last lia.
-    (* Subgoal: [load (a !!! i)] *)
-    iPoseProof (big_sepLZ2_lookup_seg_acc i with "Hslice")
-      as "(Hl & Hslice)"; try lia.
-    iApply (imp_load' with "Hl").
-    iIntros "!> !> Hl".
-    iApply "Hlookup".
-    iSplit. { iPureIntro; apply Hlen. }
-    iApply ("Hslice" with "Hl").
+    - iApply (imp_as_array_isArray a ls (Φ := λ ls', ⌜ls' = ls⌝%I) with "Ha He1"). auto.
+    - iApply (imp_as_int with "He2").
+    - iIntros (? i) "-> HΦ2".
+      iDestruct ("P" with "HΦ2") as
+        "(%dq & %j & %xs & >(%le & %Hlt & Hslice) & Hlookup)".
+      iDestruct "Hslice" as "(% & #Ha' & %Hbound & %Hle & Hslice)".
+      iPoseProof (isArray_valid with "Ha Ha'") as "->".
+      iDestruct "Ha" as "(%t & Ha & %Hlen)".
+
+      simpl.
+      rewrite signed_repr; last representable.
+      rewrite list_lookup_lookup_total_valid; last lia.
+      (* Subgoal: [load (a !!! i)] *)
+      iPoseProof (big_sepLZ2_lookup_seg_acc i with "Hslice")
+        as "(Hl & Hslice)"; try lia.
+      iApply (imp_load' with "Hl").
+      iIntros "!> !> Hl".
+      iApply "Hlookup". iFrame "#%".
+      iApply ("Hslice" with "Hl").
   Qed.
 
-  Lemma imp_EArrayGet `{Encode A, Inhabited A} {ζ} a (n : Z) (i j : Z) dq (xs : list A) x e1 e2 :
+  Lemma imp_EArrayGet' `{Encode A, Inhabited A} {ζ} a (ls : list loc) (i j : Z) dq (xs : list A) e1 e2 :
     ⌜j ≤ i⌝ -∗
     ⌜i - j < length xs⌝ -∗
-    ⌜xs !!! (i - j) = x⌝ -∗
-    isArray a n -∗
+    isArray a ls -∗
     ▷ a ↦∗[j]{dq} xs -∗
     imp eval η e1 @ E <|Ψ|> ⟨⟨ ζ ⟩⟩ {{ λ a', ⌜a' = a⌝ }} -∗
     imp eval η e2 @ E <|Ψ|> ⟨⟨ ζ ⟩⟩ {{ λ i', ⌜i' = i⌝ }} -∗
     imp eval η (EArrayGet e1 e2) @ E <|Ψ|> ⟨⟨ ζ ⟩⟩
-      {{ λ v, ⌜v = x⌝ ∗ a ↦∗[j]{dq} xs }}.
+      {{ λ (x : A), ⌜x = xs !!! (i - j)⌝ ∗ a ↦∗[j]{dq} xs }}.
   Proof.
-    iIntros (Hi Hlookup Hlen) "#Harr Hslice He1 He2".
-    iApply (imp_EArrayGet2 with "He1 He2").
-    iIntros (? ?) "-> ->".
-    iFrame "#".
-    iFrame "%". iFrame.
-    iIntros "!> $".
+    iIntros (Hi Hlen) "#Harr Hslice He1 He2".
+    iApply (imp_EArrayGet2 with "Harr He1 He2").
+    iIntros (?) "->".
+    iFrame "∗%".
+    iIntros "!> $ //".
+  Qed.
+
+    Lemma imp_EArrayGet `{Encode A, Inhabited A} {ζ} (a : array) (i j : Z) dq (xs : list A) e1 e2 :
+    ⌜0 ≤ i < length xs⌝ -∗
+    a ↦∗{dq} xs -∗
+    imp eval η e1 @ E <|Ψ|> ⟨⟨ ζ ⟩⟩ {{ λ a', ⌜a' = a⌝ }} -∗
+    imp eval η e2 @ E <|Ψ|> ⟨⟨ ζ ⟩⟩ {{ λ i', ⌜i' = i⌝ }} -∗
+    imp eval η (EArrayGet e1 e2) @ E <|Ψ|> ⟨⟨ ζ ⟩⟩
+      {{ λ (x : A), ⌜x = xs !!! i⌝ ∗ a ↦∗{dq} xs }}.
+  Proof.
+    iIntros (Hlen) "(%ls & #Harr & Hslice & %Hlenls) He1 He2".
+    iApply (imp_wand with "[-]").
+    iApply (imp_EArrayGet' with "[] [] Harr Hslice He1 He2").
+    - iPureIntro; lia.
+    - iPureIntro; lia.
+    - iIntros (x) "(-> & Hslice)".
+      iSplit.
+      + iPureIntro. rewrite Z.sub_0_r. reflexivity.
+      + iFrame "∗#%".
   Qed.
 
   Lemma imp_EArraySet2 `{Encode A, Inhabited A} {Φ : unit → iProp Σ} {ζ}
-    (Φ3 : A → iProp Σ) (Φ1 : array → iProp Σ) (Φ2 : Z → iProp Σ) e1 e2 e3 :
-    imp eval η e1 @ E <|Ψ|> ⟨⟨ ζ ⟩⟩ {{ λ a, Φ1 a }} -∗
-    imp eval η e2 @ E <|Ψ|> ⟨⟨ ζ ⟩⟩ {{ λ i, Φ2 i }} -∗
+    (Φ3 : A → iProp Σ) (Φ1 : array → list loc → iProp Σ) (Φ2 : Z → iProp Σ) e1 e2 e3 :
+    imp eval η e1 @ E <|Ψ|> ⟨⟨ ζ ⟩⟩ {{ λ a, ∃ ls, isArray a ls ∗ Φ1 a ls }} -∗
+    imp eval η e2 @ E <|Ψ|> ⟨⟨ ζ ⟩⟩ {{ Φ2 }} -∗
     imp eval η e3 @ E <|Ψ|> ⟨⟨ ζ ⟩⟩ {{ Φ3  }} -∗
-    (∀ a i y, Φ1 a -∗ Φ2 i -∗ Φ3 y -∗
-              ∃ n, isArray a n ∗
-                   ∃ j xs,
-                     ▷ (⌜j ≤ i⌝ ∗ ⌜i - j < length xs⌝ ∗ a ↦∗[j] xs) ∗
-                     ▷ (a ↦∗[j] (<[i - j := y]> xs) -∗ Φ ())) -∗
+    (∀ a ls i y, Φ1 a ls -∗ Φ2 i -∗ Φ3 y -∗
+                 ∃ j xs,
+                   ▷ (⌜j ≤ i⌝ ∗ ⌜i - j < length xs⌝ ∗ a ↦∗[j] xs) ∗
+                   ▷ (a ↦∗[j] (<[i - j := y]> xs) -∗ Φ ())) -∗
     imp eval η (EArraySet e1 e2 e3) @ E <|Ψ|> ⟨⟨ ζ ⟩⟩ {{ Φ }}.
   Proof.
     iIntros "He1 He2 He3 P". simpl_eval.
     iApply (imp_bind_par (A2:=(Z * A)) with "[He1] [He2 He3]").
-    { iApply (imp_as_array with "He1"). }
+    { set_postcondition (λ ls, ∃ a, isArray a ls ∗ Φ1 a ls)%I.
+      iApply (imp_as_array with "He1").
+      iIntros (l) "(% & #$ & $)". }
     { iApply (imp_par with "[He2] He3").
       iApply (imp_as_int with "He2"). }
-    iIntros (a (i & y)) "HΦ1 (HΦ2 & HΦ3)".
+    iIntros (ls (i & y)) "(%a & #Ha & HΦ1) (HΦ2 & HΦ3)".
     iDestruct ("P" with "HΦ1 HΦ2 HΦ3")
-      as "(%n & #Harr & %j & %xs & >(%Hle & %Hlt & Hslice) & HΦ)".
-    iDestruct "Harr" as "(%Hlen' & %Hbound)".
-    iDestruct "Hslice" as "(%Hlen & Hslice)".
+      as "(%j & %xs & >(%Hle & %Hlt & Hslice) & HΦ)".
+
+    iDestruct "Hslice" as "(% & #Ha' & %Hpos & %Hlen & Hslice)".
+    iPoseProof (isArray_valid with "Ha Ha'") as "->".
+
+    iDestruct "Ha" as "(% & _ & %Hlen')".
     simpl.
     rewrite signed_repr; last representable.
     rewrite list_lookup_lookup_total_valid; last lia.
@@ -310,18 +408,17 @@ Section array_reasoning.
 
     iApply (imp_store' with "Hl").
     iIntros "!> !> Hl".
-    iApply "HΦ".
-    iSplit; length. { iPureIntro. apply Hlen. }
+    iApply "HΦ". iFrame "Ha'". length. iFrame "%".
     iSpecialize ("Hslice" with "Hl").
     update.
     iApply "Hslice".
   Qed.
 
-  Lemma imp_EArraySet `{Encode A, Inhabited A} {ζ}
-    (Φ : A → iProp Σ) (i j n : Z) (a : array) xs e1 e2 e3 :
+  Lemma imp_EArraySet' `{Encode A, Inhabited A} {ζ}
+    (Φ : A → iProp Σ) (i j : Z) (a : array) (ls : list loc) xs e1 e2 e3 :
     ⌜j ≤ i⌝ -∗
     ⌜i - j < length xs⌝ -∗
-    isArray a n -∗
+    isArray a ls -∗
     ▷ a ↦∗[j] xs -∗
     imp eval η e1 @ E <|Ψ|> ⟨⟨ ζ ⟩⟩ {{ λ a', ⌜a'=a⌝ }} -∗
     imp eval η e2 @ E <|Ψ|> ⟨⟨ ζ ⟩⟩ {{ λ i', ⌜i'=i⌝ }} -∗
@@ -330,13 +427,38 @@ Section array_reasoning.
       {{ λ (_ : unit), ∃ y, Φ y ∗ a ↦∗[j] (<[i-j:=y]> xs) }}.
   Proof.
     iIntros (Hbound Hlen) "#Harr Hslice He1 He2 He3".
-    iApply (imp_EArraySet2 with "He1 He2 He3").
-    iIntros (?? y) "-> -> HΦ".
-    iFrame "#". iFrame.
+    iApply (imp_EArraySet2 with "[He1] He2 He3").
+    { set_postcondition (λ a', ∃ ls', _ ∗ ⌜a' = a⌝ ∗ ⌜ls' = ls⌝)%I.
+      iApply (imp_wand with "He1").
+      iIntros (?) "->". iFrame "Harr". auto. }
+    iIntros (??? y) "(-> & ->) -> HΦ".
+    iFrame.
     iSplit.
     - iPureIntro. lia.
     - iIntros "!> Hslice".
       iFrame.
+  Qed.
+
+  Lemma imp_EArraySet `{Encode A, Inhabited A} {ζ}
+    (Φ : A → iProp Σ) (i j : Z) (a : array) xs e1 e2 e3 :
+    ⌜0 ≤ i < length xs⌝ -∗
+    a ↦∗ xs -∗
+    imp eval η e1 @ E <|Ψ|> ⟨⟨ ζ ⟩⟩ {{ λ a', ⌜a'=a⌝ }} -∗
+    imp eval η e2 @ E <|Ψ|> ⟨⟨ ζ ⟩⟩ {{ λ i', ⌜i'=i⌝ }} -∗
+    imp eval η e3 @ E <|Ψ|> ⟨⟨ ζ ⟩⟩ {{ Φ }} -∗
+    imp eval η (EArraySet e1 e2 e3) @ E <|Ψ|> ⟨⟨ ζ ⟩⟩
+      {{ λ (_ : unit), ∃ y, Φ y ∗ a ↦∗ (<[i:=y]> xs) }}.
+  Proof.
+    iIntros (Hbound) "Harr He1 He2 He3".
+    iDestruct "Harr" as "(%ls & #Ha & Hslice & %Hlen)".
+    iApply (imp_wand with "[-]").
+    iApply (imp_EArraySet' with "[] [] Ha Hslice He1 He2 He3").
+    - iPureIntro; lia.
+    - iPureIntro; lia.
+    - iIntros ([]) "(%y & $ & Hslice)".
+      rewrite Z.sub_0_r.
+      iApply (isSlice_ownArray with "Ha Hslice").
+      by length.
   Qed.
 
 End array_reasoning.
